calc_sample/impl/Calc.Server.CanonicalProtocol.fst
@@ -1,0 +1,1054 @@
+module Calc.Server.CanonicalProtocol
+
+#lang-pulse
+
+open Pulse.Lib.Pervasives
+
+module CPI = Common.ProtocolImplementation
+module ID = FStar.IndefiniteDescription
+module L = FStar.List.Tot
+module LP = FStar.List.Tot.Properties
+module MR = Pulse.Lib.MonotonicGhostRef
+module Pre = FStar.Preorder
+module RTC = FStar.ReflexiveTransitiveClosure
+module Seq = FStar.Seq
+module SM = Common.StateMachine
+module SZ = FStar.SizeT
+module TCP = Common.TCP
+module WF = Common.WireFormat
+module WFSM = Common.WireFormatStateMachine
+module U8 = FStar.UInt8
+module Vec = Pulse.Lib.Vec
+
+module CalcParser = Calc.Impl.Parser
+module CalcP = Calc.Protocol
+
+open Calc.Log
+open Calc.Wire
+open Calc.Impl.Types
+
+let calc_server_step_rel
+  (log0:calc_log)
+  (log1:calc_log)
+  : prop =
+  exists msg.
+    CalcP.calc_frame_network_step_ok
+      log0
+      msg
+      log1
+      (CalcP.calc_frame_response_for log0 msg)
+
+let calc_server_state_ahead_preorder
+  : Pre.preorder calc_log =
+  RTC.closure calc_server_step_rel
+
+let calc_server_transition
+  (log0:calc_log)
+  (msg:CalcP.calc_frame)
+  (log1:calc_log)
+  : SM.transition calc_log CalcP.calc_frame CalcP.calc_frame_local_event unit =
+  let output = {
+    SM.so_wire_outputs = [CalcP.calc_frame_response_for log0 msg];
+    SM.so_local_outputs = [];
+  } in
+  {
+    SM.tr_event = SM.WireEvent msg;
+    SM.tr_next_state = log1;
+    SM.tr_output = output;
+  }
+
+let lemma_calc_server_step_rel_state_ahead
+  (log0:calc_log)
+  (log1:calc_log)
+  : Lemma
+      (requires calc_server_step_rel log0 log1)
+      (ensures
+        CPI.state_ahead
+          CalcP.calc_frame_wire_format_state_machine
+          log0
+          log1)
+=
+  let msg =
+    FStar.IndefiniteDescription.indefinite_description_ghost
+      CalcP.calc_frame
+      (fun msg ->
+        CalcP.calc_frame_network_step_ok
+          log0
+          msg
+          log1
+          (CalcP.calc_frame_response_for log0 msg)) in
+  let tr = calc_server_transition log0 msg log1 in
+  assert (SM.trace_reaches
+    CalcP.calc_frame_wire_format_state_machine.WFSM.wfsm_state_machine
+    log0
+    [tr]
+    log1);
+  assert (exists trace.
+    SM.trace_reaches
+      CalcP.calc_frame_wire_format_state_machine.WFSM.wfsm_state_machine
+      log0
+      trace
+      log1)
+
+let lemma_calc_server_closure_state_ahead
+  (log0:calc_log)
+  (log1:calc_log)
+  : Lemma
+      (requires calc_server_state_ahead_preorder log0 log1)
+      (ensures
+        CPI.state_ahead
+          CalcP.calc_frame_wire_format_state_machine
+          log0
+          log1)
+=
+  RTC.induct
+    calc_server_step_rel
+    (fun x y ->
+      CPI.state_ahead
+        CalcP.calc_frame_wire_format_state_machine
+        x
+        y)
+    (fun x ->
+      SM.lemma_state_evolves_refl
+        CalcP.calc_frame_wire_format_state_machine.WFSM.wfsm_state_machine
+        x)
+    (fun x y ->
+      lemma_calc_server_step_rel_state_ahead x y)
+    (fun x y z ->
+      SM.lemma_state_evolves_trans
+        CalcP.calc_frame_wire_format_state_machine.WFSM.wfsm_state_machine
+        x
+        y
+        z)
+    log0
+    log1
+    ()
+
+let lemma_calc_valid_initial ()
+  : Lemma
+      (ensures
+        WFSM.valid_byte_trace
+          CalcP.calc_frame_wire_format_state_machine
+          Seq.empty
+          initial_log
+          Seq.empty
+          Seq.empty)
+=
+  assert (SM.trace_reaches
+    CalcP.calc_frame_wire_format_state_machine.WFSM.wfsm_state_machine
+    initial_log
+    []
+    initial_log);
+  assert (WF.parses_as CalcP.calc_frame_wire_format Seq.empty [] Seq.empty);
+  assert (Seq.equal Seq.empty (WF.serialize_all CalcP.calc_frame_wire_format []));
+  let trace = [] in
+  assert (
+    SM.trace_reaches
+      CalcP.calc_frame_wire_format_state_machine.WFSM.wfsm_state_machine
+      CalcP.calc_frame_wire_format_state_machine.WFSM.wfsm_state_machine.SM.sm_initial_state
+      trace
+      initial_log /\
+    WF.parses_as
+      CalcP.calc_frame_wire_format
+      Seq.empty
+      (WFSM.trace_input_messages trace)
+      Seq.empty /\
+    Seq.equal
+      Seq.empty
+      (WF.serialize_all
+        CalcP.calc_frame_wire_format
+        (SM.trace_wire_outputs trace)));
+  assert (exists trace.
+    SM.trace_reaches
+      CalcP.calc_frame_wire_format_state_machine.WFSM.wfsm_state_machine
+      CalcP.calc_frame_wire_format_state_machine.WFSM.wfsm_state_machine.SM.sm_initial_state
+      trace
+      initial_log /\
+    WF.parses_as
+      CalcP.calc_frame_wire_format
+      Seq.empty
+      (WFSM.trace_input_messages trace)
+      Seq.empty /\
+    Seq.equal
+      Seq.empty
+      (WF.serialize_all
+        CalcP.calc_frame_wire_format
+        (SM.trace_wire_outputs trace)))
+
+noeq
+type canonical_server = {
+  canonical_server_state: server_state;
+  canonical_server_progress: MR.mref calc_server_state_ahead_preorder;
+}
+
+let canonical_trace_witness
+  (received:TCP.bytes)
+  (sent:TCP.bytes)
+  (log:calc_log)
+  (trace:list (SM.transition calc_log CalcP.calc_frame CalcP.calc_frame_local_event unit))
+  : prop =
+  SM.trace_reaches
+    CalcP.calc_frame_wire_format_state_machine.WFSM.wfsm_state_machine
+    initial_log
+    trace
+    log /\
+  Seq.equal
+    received
+    (WF.serialize_all
+      CalcP.calc_frame_wire_format
+      (WFSM.trace_input_messages trace)) /\
+  Seq.equal
+    sent
+    (WF.serialize_all
+      CalcP.calc_frame_wire_format
+      (SM.trace_wire_outputs trace)) /\
+  Seq.equal received log.input_bytes /\
+  Seq.equal sent log.output_bytes
+
+let canonical_trace_ok
+  (received:TCP.bytes)
+  (sent:TCP.bytes)
+  (log:calc_log)
+  : prop =
+  exists trace. canonical_trace_witness received sent log trace
+
+let lemma_canonical_trace_ok_valid
+  (received:TCP.bytes)
+  (sent:TCP.bytes)
+  (log:calc_log)
+  : Lemma
+      (requires canonical_trace_ok received sent log)
+      (ensures
+        WFSM.valid_byte_trace
+          CalcP.calc_frame_wire_format_state_machine
+          received
+          log
+          sent
+          Seq.empty)
+=
+  let trace =
+    ID.indefinite_description_ghost
+      (list (SM.transition calc_log CalcP.calc_frame CalcP.calc_frame_local_event unit))
+      (canonical_trace_witness received sent log) in
+  assert (canonical_trace_witness received sent log trace);
+  WF.lemma_parse_serialize_all_inverse
+    CalcP.calc_frame_wire_format
+    CalcP.calc_frame_wire_format_stream_laws
+    (WFSM.trace_input_messages trace);
+  Seq.lemma_eq_elim
+    received
+    (WF.serialize_all
+      CalcP.calc_frame_wire_format
+      (WFSM.trace_input_messages trace));
+  assert (
+    WF.parses_as
+      CalcP.calc_frame_wire_format
+      received
+      (WFSM.trace_input_messages trace)
+      Seq.empty);
+  assert (exists trace'.
+    SM.trace_reaches
+      CalcP.calc_frame_wire_format_state_machine.WFSM.wfsm_state_machine
+      CalcP.calc_frame_wire_format_state_machine.WFSM.wfsm_state_machine.SM.sm_initial_state
+      trace'
+      log /\
+    WF.parses_as
+      CalcP.calc_frame_wire_format
+      received
+      (WFSM.trace_input_messages trace')
+      Seq.empty /\
+    Seq.equal
+      sent
+      (WF.serialize_all
+        CalcP.calc_frame_wire_format
+        (SM.trace_wire_outputs trace')))
+
+let lemma_canonical_trace_ok_network_step
+  (received0:TCP.bytes)
+  (sent0:TCP.bytes)
+  (log0:calc_log)
+  (msg:CalcP.calc_frame)
+  (log1:calc_log)
+  (actual_output:TCP.bytes)
+  : Lemma
+      (requires
+        canonical_trace_ok received0 sent0 log0 /\
+        CalcP.calc_frame_network_step_ok log0 msg log1 actual_output)
+      (ensures
+        canonical_trace_ok
+          (Seq.append received0 msg)
+          (Seq.append sent0 actual_output)
+          log1)
+=
+  let trace0 =
+    ID.indefinite_description_ghost
+      (list (SM.transition calc_log CalcP.calc_frame CalcP.calc_frame_local_event unit))
+      (canonical_trace_witness received0 sent0 log0) in
+  assert (canonical_trace_witness received0 sent0 log0 trace0);
+  let response_msg = CalcP.calc_frame_response_for log0 msg in
+  let tr = calc_server_transition log0 msg log1 in
+  assert (
+    CalcP.calc_frame_step
+      log0
+      (SM.WireEvent msg)
+      log1
+      tr.SM.tr_output);
+  assert (SM.trace_reaches
+    CalcP.calc_frame_wire_format_state_machine.WFSM.wfsm_state_machine
+    log0
+    [tr]
+    log1);
+  SM.lemma_trace_reaches_append
+    CalcP.calc_frame_wire_format_state_machine.WFSM.wfsm_state_machine
+    initial_log
+    log0
+    log1
+    trace0
+    [tr];
+  CalcP.lemma_calc_trace_input_bytes_append_one trace0 tr;
+  CalcP.lemma_calc_trace_wire_bytes_append_one trace0 tr;
+  Seq.append_empty_r msg;
+  Seq.append_empty_r response_msg;
+  assert (Seq.equal
+    (WF.serialize_all
+      CalcP.calc_frame_wire_format
+      (WFSM.trace_input_messages (L.append trace0 [tr])))
+    (Seq.append
+      (WF.serialize_all
+        CalcP.calc_frame_wire_format
+        (WFSM.trace_input_messages trace0))
+      msg));
+  assert (Seq.equal
+    (WF.serialize_all
+      CalcP.calc_frame_wire_format
+      (SM.trace_wire_outputs (L.append trace0 [tr])))
+    (Seq.append
+      (WF.serialize_all
+        CalcP.calc_frame_wire_format
+        (SM.trace_wire_outputs trace0))
+      response_msg));
+  Seq.lemma_eq_elim
+    received0
+    (WF.serialize_all
+      CalcP.calc_frame_wire_format
+      (WFSM.trace_input_messages trace0));
+  Seq.lemma_eq_elim
+    sent0
+    (WF.serialize_all
+      CalcP.calc_frame_wire_format
+      (SM.trace_wire_outputs trace0));
+  Seq.lemma_eq_elim response_msg actual_output;
+  assert (Seq.equal
+    (Seq.append received0 msg)
+    (WF.serialize_all
+      CalcP.calc_frame_wire_format
+      (WFSM.trace_input_messages (L.append trace0 [tr]))));
+  assert (Seq.equal
+    (Seq.append sent0 actual_output)
+    (WF.serialize_all
+      CalcP.calc_frame_wire_format
+      (SM.trace_wire_outputs (L.append trace0 [tr]))));
+  assert (Seq.equal (Seq.append received0 msg) log1.input_bytes);
+  assert (Seq.equal (Seq.append sent0 actual_output) log1.output_bytes);
+  assert (canonical_trace_witness
+    (Seq.append received0 msg)
+    (Seq.append sent0 actual_output)
+    log1
+    (L.append trace0 [tr]));
+  assert (exists trace.
+    canonical_trace_witness
+      (Seq.append received0 msg)
+      (Seq.append sent0 actual_output)
+      log1
+      trace)
+
+noeq
+type calc_network_frame = {
+  calc_network_req: Vec.vec U8.t;
+  calc_network_resp: Vec.vec U8.t;
+}
+
+type calc_local_frame = unit
+
+[@inline_let]
+let calc_process_result
+  (status:CPI.process_status)
+  (consumed:SZ.t)
+  (produced:SZ.t)
+  : CPI.process_result =
+  {
+    CPI.process_status = status;
+    CPI.process_consumed_len = consumed;
+    CPI.process_produced_len = produced;
+    CPI.process_app_len = 0sz;
+  }
+
+[@inline_let]
+let calc_step_ok_result : CPI.process_result =
+  calc_process_result CPI.StepOk 5sz 5sz
+
+let calc_need_more_input_result : CPI.process_result =
+  calc_process_result CPI.NeedMoreInput 0sz 0sz
+
+let calc_parse_failed_result : CPI.process_result =
+  calc_process_result CPI.ParseFailed 0sz 0sz
+
+let calc_no_local_outputs : list unit = []
+
+let empty_calc_trace
+  : list (SM.transition calc_log CalcP.calc_frame CalcP.calc_frame_local_event unit)
+  = []
+
+let default_calc_frame : CalcP.calc_frame =
+  CalcP.calc_response_frame Error
+
+let calc_frame_or_default
+  (b:TCP.bytes)
+  : GTot CalcP.calc_frame =
+  if Seq.length b == 5 then
+    match parse_request b with
+    | Some _ -> b
+    | None -> default_calc_frame
+  else
+    default_calc_frame
+
+let lemma_calc_frame_or_default_valid
+  (b:TCP.bytes{Seq.length b == 5 /\ parse_request b <> None})
+  : Lemma
+      (ensures calc_frame_or_default b == b)
+=
+  match parse_request b with
+  | Some _ -> ()
+
+let lemma_network_process_correct_step_ok
+  (input:TCP.bytes)
+  (input_len:SZ.t)
+  (old_out:TCP.bytes)
+  (out_bytes:TCP.bytes)
+  (out_len:SZ.t)
+  (received0:TCP.bytes)
+  (sent0:TCP.bytes)
+  (log0:calc_log)
+  (received1:TCP.bytes)
+  (sent1:TCP.bytes)
+  (log1:calc_log)
+  (consumed:TCP.bytes)
+  (wire_outputs:list CalcP.calc_frame)
+  (local_outputs:list unit)
+  (produced:TCP.bytes)
+  : Lemma
+      (requires
+        CPI.buffers_wf input input_len old_out out_len /\
+        Seq.length out_bytes == Seq.length old_out /\
+        CPI.consumed_by_parse
+          CalcP.calc_frame_wire_format
+          (CPI.input_bytes input input_len)
+          (calc_frame_or_default input)
+          consumed
+          Seq.empty /\
+        SZ.v calc_step_ok_result.CPI.process_consumed_len == Seq.length consumed /\
+        CalcP.calc_frame_wire_format_state_machine.WFSM.wfsm_state_machine.SM.sm_step
+          log0
+          (SM.WireEvent (calc_frame_or_default input))
+          log1
+          (CPI.step_output wire_outputs local_outputs) /\
+        Seq.equal
+          produced
+          (WF.serialize_all CalcP.calc_frame_wire_format wire_outputs) /\
+        CPI.output_written
+          out_bytes
+          calc_step_ok_result.CPI.process_produced_len
+          produced /\
+        Seq.equal received1 (Seq.append received0 consumed) /\
+        Seq.equal sent1 (Seq.append sent0 produced))
+      (ensures
+        CPI.network_process_correct
+          CalcP.calc_frame_wire_format_state_machine
+          input
+          input_len
+          old_out
+          out_bytes
+          out_len
+          received0
+          sent0
+          log0
+          calc_step_ok_result
+          received1
+          sent1
+          log1
+          consumed
+          wire_outputs
+          local_outputs)
+=
+  let msg = calc_frame_or_default input in
+  assert (CPI.consumed_by_parse
+    CalcP.calc_frame_wire_format
+    (CPI.input_bytes input input_len)
+    msg
+    consumed
+    Seq.empty);
+  assert (SZ.v calc_step_ok_result.CPI.process_consumed_len == Seq.length consumed);
+  assert (CalcP.calc_frame_wire_format_state_machine.WFSM.wfsm_state_machine.SM.sm_step
+    log0
+    (SM.WireEvent msg)
+    log1
+    (CPI.step_output wire_outputs local_outputs));
+  assert (Seq.equal
+    produced
+    (WF.serialize_all CalcP.calc_frame_wire_format wire_outputs));
+  assert (CPI.output_written
+    out_bytes
+    calc_step_ok_result.CPI.process_produced_len
+    produced);
+  assert (Seq.equal received1 (Seq.append received0 consumed));
+  assert (Seq.equal sent1 (Seq.append sent0 produced));
+  assert_norm (calc_step_ok_result.CPI.process_status == CPI.StepOk);
+  assert (calc_step_ok_result.CPI.process_status == CPI.StepOk);
+  assert (exists msg' residual produced'.
+    CPI.consumed_by_parse
+      CalcP.calc_frame_wire_format
+      (CPI.input_bytes input input_len)
+      msg'
+      consumed
+      residual /\
+    SZ.v calc_step_ok_result.CPI.process_consumed_len == Seq.length consumed /\
+    CalcP.calc_frame_wire_format_state_machine.WFSM.wfsm_state_machine.SM.sm_step
+      log0
+      (SM.WireEvent msg')
+      log1
+      (CPI.step_output wire_outputs local_outputs) /\
+    Seq.equal
+      produced'
+      (WF.serialize_all CalcP.calc_frame_wire_format wire_outputs) /\
+    CPI.output_written
+      out_bytes
+      calc_step_ok_result.CPI.process_produced_len
+      produced' /\
+    Seq.equal received1 (Seq.append received0 consumed) /\
+    Seq.equal sent1 (Seq.append sent0 produced'));
+  assert (5 == Seq.length consumed);
+  assert (CPI.output_written out_bytes 5sz produced);
+  assert (Seq.equal
+    produced
+    (WF.serialize_all
+      CalcP.calc_frame_wire_format_state_machine.WFSM.wfsm_wire_format
+      wire_outputs));
+  assert (exists msg' residual produced'.
+    CPI.consumed_by_parse
+      CalcP.calc_frame_wire_format_state_machine.WFSM.wfsm_wire_format
+      (CPI.input_bytes input input_len)
+      msg'
+      consumed
+      residual /\
+    5 == Seq.length consumed /\
+    CalcP.calc_frame_wire_format_state_machine.WFSM.wfsm_state_machine.SM.sm_step
+      log0
+      (SM.WireEvent msg')
+      log1
+      (CPI.step_output wire_outputs local_outputs) /\
+    Seq.equal
+      produced'
+      (WF.serialize_all
+        CalcP.calc_frame_wire_format_state_machine.WFSM.wfsm_wire_format
+        wire_outputs) /\
+    CPI.output_written out_bytes 5sz produced' /\
+    Seq.equal received1 (Seq.append received0 consumed) /\
+    Seq.equal sent1 (Seq.append sent0 produced'));
+  match calc_step_ok_result.CPI.process_status with
+  | CPI.StepOk ->
+    assert (CPI.network_process_correct
+      CalcP.calc_frame_wire_format_state_machine
+      input
+      input_len
+      old_out
+      out_bytes
+      out_len
+      received0
+      sent0
+      log0
+      calc_step_ok_result
+      received1
+      sent1
+      log1
+      consumed
+      wire_outputs
+      local_outputs)
+    by (
+      FStar.Tactics.norm
+        [delta_only
+          [`%CPI.network_process_correct;
+           `%calc_step_ok_result;
+           `%calc_process_result;
+           `%Common.ProtocolImplementation.__proj__Mkprocess_result__item__process_status;
+           `%Common.ProtocolImplementation.__proj__Mkprocess_result__item__process_consumed_len;
+           `%Common.ProtocolImplementation.__proj__Mkprocess_result__item__process_produced_len];
+         iota; zeta; primops];
+      FStar.Tactics.smt ())
+  | _ ->
+    assert False
+
+let canonical_server_exactly
+  (srv:canonical_server)
+  (received:TCP.bytes)
+  (sent:TCP.bytes)
+  (log:calc_log)
+  : slprop =
+  server_exactly srv.canonical_server_state log **
+  MR.pts_to srv.canonical_server_progress #1.0R log **
+  pure (canonical_trace_ok received sent log)
+
+let canonical_server_snapshot
+  (srv:canonical_server)
+  (_received:TCP.bytes)
+  (_sent:TCP.bytes)
+  (log:calc_log)
+  : slprop =
+  MR.snapshot srv.canonical_server_progress log
+
+[@@pulse_unfold]
+let calc_network_frame_pre
+  (frame:calc_network_frame)
+  (input:array U8.t)
+  (input_len:SZ.t)
+  (out:array U8.t)
+  (out_len:SZ.t)
+  (input_contents:TCP.bytes)
+  (old_out:TCP.bytes)
+  : slprop =
+  pure (
+    input == Vec.vec_to_array frame.calc_network_req /\
+    out == Vec.vec_to_array frame.calc_network_resp /\
+    Seq.length input_contents == 5 /\
+    Seq.length old_out == 5 /\
+    input_len == 5sz /\
+    parse_request input_contents <> None /\
+    out_len == 5sz)
+
+let calc_network_frame_post
+  (_frame:calc_network_frame)
+  (result:CPI.process_result)
+  (input_contents:TCP.bytes)
+  (_input_len:SZ.t)
+  (_old_out:TCP.bytes)
+  (out_contents:TCP.bytes)
+  (st0:calc_log)
+  (st1:calc_log)
+  (consumed:TCP.bytes)
+  (wire_outputs:list CalcP.calc_frame)
+  (local_outputs:list unit)
+  : slprop =
+  let msg = calc_frame_or_default input_contents in
+  let response_msg = CalcP.calc_frame_response_for st0 msg in
+  pure (
+    result == calc_step_ok_result /\
+    consumed == input_contents /\
+    wire_outputs == [response_msg] /\
+    local_outputs == [] /\
+    CalcP.calc_frame_network_step_ok st0 msg st1 out_contents)
+
+[@@pulse_unfold]
+let calc_local_frame_pre
+  (_ev:CalcP.calc_frame_local_event)
+  (_frame:calc_local_frame)
+  (_st0:calc_log)
+  (_out:array U8.t)
+  (_out_len:SZ.t)
+  (_old_out:TCP.bytes)
+  : slprop =
+  emp
+
+let calc_local_frame_post
+  (_ev:CalcP.calc_frame_local_event)
+  (_frame:calc_local_frame)
+  (result:CPI.process_result)
+  (old_out:TCP.bytes)
+  (out_contents:TCP.bytes)
+  (st0:calc_log)
+  (st1:calc_log)
+  (wire_outputs:list CalcP.calc_frame)
+  (local_outputs:list unit)
+  : slprop =
+  pure (
+    result == calc_process_result CPI.StepOk 0sz 0sz /\
+    out_contents == old_out /\
+    st1 == st0 /\
+    wire_outputs == [] /\
+    local_outputs == [])
+
+fn calc_invariant_valid
+  (srv:canonical_server)
+  (received:erased TCP.bytes)
+  (sent:erased TCP.bytes)
+  (log:erased calc_log)
+requires canonical_server_exactly srv received sent log
+ensures
+  canonical_server_exactly srv received sent log **
+  pure (
+    WFSM.valid_byte_trace
+      CalcP.calc_frame_wire_format_state_machine
+      received
+      log
+      sent
+      Seq.empty)
+{
+  unfold (canonical_server_exactly srv received sent log);
+  lemma_canonical_trace_ok_valid received sent log;
+  assert (pure (WFSM.valid_byte_trace
+    CalcP.calc_frame_wire_format_state_machine
+    received
+    log
+    sent
+    Seq.empty));
+  fold (canonical_server_exactly srv received sent log)
+}
+
+fn calc_take_snapshot
+  (srv:canonical_server)
+  (received:erased TCP.bytes)
+  (sent:erased TCP.bytes)
+  (log:erased calc_log)
+requires canonical_server_exactly srv received sent log
+ensures
+  canonical_server_exactly srv received sent log **
+  canonical_server_snapshot srv received sent log
+{
+  unfold (canonical_server_exactly srv received sent log);
+  MR.take_snapshot srv.canonical_server_progress log;
+  fold (canonical_server_snapshot srv received sent log);
+  fold (canonical_server_exactly srv received sent log)
+}
+
+fn calc_recall_snapshot
+  (srv:canonical_server)
+  (snapshot_received:erased TCP.bytes)
+  (snapshot_sent:erased TCP.bytes)
+  (snapshot_log:erased calc_log)
+  (current_received:erased TCP.bytes)
+  (current_sent:erased TCP.bytes)
+  (current_log:erased calc_log)
+requires
+  canonical_server_snapshot srv snapshot_received snapshot_sent snapshot_log **
+  canonical_server_exactly srv current_received current_sent current_log
+ensures
+  canonical_server_snapshot srv snapshot_received snapshot_sent snapshot_log **
+  canonical_server_exactly srv current_received current_sent current_log **
+  pure (
+    CPI.state_ahead
+      CalcP.calc_frame_wire_format_state_machine
+      snapshot_log
+      current_log)
+{
+  unfold (canonical_server_snapshot srv snapshot_received snapshot_sent snapshot_log);
+  unfold (canonical_server_exactly srv current_received current_sent current_log);
+  MR.recall_snapshot srv.canonical_server_progress;
+  lemma_calc_server_closure_state_ahead snapshot_log current_log;
+  fold (canonical_server_snapshot srv snapshot_received snapshot_sent snapshot_log);
+  fold (canonical_server_exactly srv current_received current_sent current_log)
+}
+
+fn calc_process_network
+  (srv:canonical_server)
+  (frame:calc_network_frame)
+  (input:array U8.t)
+  (input_len:SZ.t)
+  (out:array U8.t)
+  (out_len:SZ.t)
+  (received0:erased TCP.bytes)
+  (sent0:erased TCP.bytes)
+  (log0:erased calc_log)
+  (input_contents:erased TCP.bytes)
+  (old_out:erased TCP.bytes)
+requires
+  canonical_server_exactly srv received0 sent0 log0 **
+  calc_network_frame_pre frame input input_len out out_len input_contents old_out **
+  pts_to input input_contents **
+  pts_to out old_out **
+  pure (CPI.buffers_wf input_contents input_len old_out out_len)
+returns result:CPI.process_result
+ensures exists* (received1:Ghost.erased TCP.bytes)
+                (sent1:Ghost.erased TCP.bytes)
+                (log1:Ghost.erased calc_log)
+                (out_contents:TCP.bytes)
+                (consumed:TCP.bytes)
+                (wire_outputs:list CalcP.calc_frame)
+                (local_outputs:list unit).
+  canonical_server_exactly srv (Ghost.reveal received1) (Ghost.reveal sent1) (Ghost.reveal log1) **
+  calc_network_frame_post
+    frame
+    result
+    input_contents
+    input_len
+    old_out
+    out_contents
+    log0
+    (Ghost.reveal log1)
+    consumed
+    wire_outputs
+    local_outputs **
+  pts_to input input_contents **
+  pts_to out out_contents **
+  pure (
+    CPI.network_process_correct
+      CalcP.calc_frame_wire_format_state_machine
+      input_contents
+      input_len
+      old_out
+      out_contents
+      out_len
+      received0
+      sent0
+      log0
+      result
+      (Ghost.reveal received1)
+      (Ghost.reveal sent1)
+      (Ghost.reveal log1)
+      consumed
+      wire_outputs
+      local_outputs)
+{
+  unfold (canonical_server_exactly srv received0 sent0 log0);
+  unfold (calc_network_frame_pre frame input input_len out out_len input_contents old_out);
+  rewrite (pts_to input input_contents) as (pts_to (Vec.vec_to_array frame.calc_network_req) input_contents);
+  rewrite (pts_to out old_out) as (pts_to (Vec.vec_to_array frame.calc_network_resp) old_out);
+  Vec.to_vec_pts_to frame.calc_network_req;
+  Vec.to_vec_pts_to frame.calc_network_resp;
+  Calc.Server.process_request srv.canonical_server_state frame.calc_network_req frame.calc_network_resp;
+  with resp_bytes1 log1. _;
+  Vec.to_array_pts_to frame.calc_network_req;
+  Vec.to_array_pts_to frame.calc_network_resp;
+  rewrite (pts_to (Vec.vec_to_array frame.calc_network_req) input_contents) as (pts_to input input_contents);
+  rewrite (pts_to (Vec.vec_to_array frame.calc_network_resp) resp_bytes1) as (pts_to out resp_bytes1);
+  let msge : erased CalcP.calc_frame = Ghost.hide (Ghost.reveal input_contents);
+  let response_msge : erased CalcP.calc_frame =
+    Ghost.hide (CalcP.calc_frame_response_for log0 (Ghost.reveal msge));
+  lemma_canonical_trace_ok_network_step received0 sent0 log0 (Ghost.reveal msge) log1 resp_bytes1;
+  assert (pure (CalcP.calc_frame_network_step_ok log0 (Ghost.reveal msge) log1 (Ghost.reveal response_msge)));
+  assert (pure (calc_server_step_rel log0 log1));
+  RTC.closure_step calc_server_step_rel log0 log1;
+  MR.update srv.canonical_server_progress log1;
+  let received1e = Ghost.hide (Seq.append received0 input_contents);
+  let sent1e = Ghost.hide (Seq.append sent0 resp_bytes1);
+  let log1e = Ghost.hide log1;
+  fold (canonical_server_exactly
+    srv
+    (Ghost.reveal received1e)
+    (Ghost.reveal sent1e)
+    (Ghost.reveal log1e));
+  lemma_calc_frame_or_default_valid input_contents;
+  fold (calc_network_frame_post
+    frame
+    calc_step_ok_result
+    input_contents
+    input_len
+    old_out
+    resp_bytes1
+    log0
+    (Ghost.reveal log1e)
+    input_contents
+    [Ghost.reveal response_msge]
+    calc_no_local_outputs);
+  CalcP.lemma_slice_full_5 (Ghost.reveal msge);
+  assert (pure (Seq.equal (CPI.input_bytes input_contents input_len) (Ghost.reveal msge)));
+  Seq.lemma_eq_elim (CPI.input_bytes input_contents input_len) (Ghost.reveal msge);
+  CalcP.lemma_calc_parse_serialize_exact (Ghost.reveal msge);
+  Seq.append_empty_r input_contents;
+  assert (pure (CPI.consumed_by_parse
+    CalcP.calc_frame_wire_format
+    (CPI.input_bytes input_contents input_len)
+    (Ghost.reveal msge)
+    input_contents
+    Seq.empty));
+  Seq.lemma_eq_elim (Ghost.reveal response_msge) resp_bytes1;
+  Seq.append_empty_r (Ghost.reveal response_msge);
+  assert (pure (Seq.equal
+    (Ghost.reveal response_msge)
+    (WF.serialize_all CalcP.calc_frame_wire_format [Ghost.reveal response_msge])));
+  assert (pure (CPI.output_written resp_bytes1 5sz (Ghost.reveal response_msge)));
+  assert (pure (SZ.v calc_step_ok_result.CPI.process_consumed_len == Seq.length input_contents));
+  assert (pure (Seq.equal (Ghost.reveal received1e) (Seq.append received0 input_contents)));
+  assert (pure (Seq.equal (Ghost.reveal sent1e) (Seq.append sent0 (Ghost.reveal response_msge))));
+  assert (pure (CalcP.calc_frame_wire_format_state_machine.WFSM.wfsm_state_machine.SM.sm_step
+    log0
+    (SM.WireEvent (Ghost.reveal msge))
+    (Ghost.reveal log1e)
+    (CPI.step_output [Ghost.reveal response_msge] calc_no_local_outputs)));
+  assert (pure (calc_step_ok_result.CPI.process_status == CPI.StepOk));
+  assert (pure (calc_step_ok_result.CPI.process_consumed_len == 5sz));
+  assert (pure (calc_step_ok_result.CPI.process_produced_len == 5sz));
+  assert (pure (CPI.buffers_wf input_contents input_len old_out out_len));
+  assert (pure (Seq.length resp_bytes1 == Seq.length old_out));
+  assert (pure (exists produced.
+    CPI.consumed_by_parse
+      CalcP.calc_frame_wire_format
+      (CPI.input_bytes input_contents input_len)
+      (Ghost.reveal msge)
+      input_contents
+      Seq.empty /\
+    SZ.v calc_step_ok_result.CPI.process_consumed_len == Seq.length input_contents /\
+    CalcP.calc_frame_wire_format_state_machine.WFSM.wfsm_state_machine.SM.sm_step
+      log0
+      (SM.WireEvent (Ghost.reveal msge))
+      (Ghost.reveal log1e)
+      (CPI.step_output [Ghost.reveal response_msge] calc_no_local_outputs) /\
+    Seq.equal
+      produced
+      (WF.serialize_all CalcP.calc_frame_wire_format [Ghost.reveal response_msge]) /\
+    CPI.output_written resp_bytes1 calc_step_ok_result.CPI.process_produced_len produced /\
+    Seq.equal (Ghost.reveal received1e) (Seq.append received0 input_contents) /\
+    Seq.equal (Ghost.reveal sent1e) (Seq.append sent0 produced)));
+  lemma_network_process_correct_step_ok
+    input_contents
+    input_len
+    old_out
+    resp_bytes1
+    out_len
+    received0
+    sent0
+    log0
+    (Ghost.reveal received1e)
+    (Ghost.reveal sent1e)
+    (Ghost.reveal log1e)
+    input_contents
+    [Ghost.reveal response_msge]
+    calc_no_local_outputs
+    (Ghost.reveal response_msge);
+  assert (pure (CPI.network_process_correct
+    CalcP.calc_frame_wire_format_state_machine
+    input_contents
+    input_len
+    old_out
+    resp_bytes1
+    out_len
+    received0
+    sent0
+    log0
+    calc_step_ok_result
+    (Ghost.reveal received1e)
+    (Ghost.reveal sent1e)
+    (Ghost.reveal log1e)
+    input_contents
+    [Ghost.reveal response_msge]
+    calc_no_local_outputs));
+  calc_step_ok_result
+}
+
+fn calc_process_local
+  (srv:canonical_server)
+  (ev:CalcP.calc_frame_local_event)
+  (frame:calc_local_frame)
+  (out:array U8.t)
+  (out_len:SZ.t)
+  (received0:erased TCP.bytes)
+  (sent0:erased TCP.bytes)
+  (log0:erased calc_log)
+  (old_out:erased TCP.bytes)
+requires
+  canonical_server_exactly srv received0 sent0 log0 **
+  calc_local_frame_pre ev frame log0 out out_len old_out **
+  pts_to out old_out **
+  pure (SZ.v out_len == Seq.length old_out)
+returns result:CPI.process_result
+ensures exists* (received1:Ghost.erased TCP.bytes)
+                (sent1:Ghost.erased TCP.bytes)
+                (log1:Ghost.erased calc_log)
+                (out_contents:TCP.bytes)
+                (wire_outputs:list CalcP.calc_frame)
+                (local_outputs:list unit).
+  canonical_server_exactly srv (Ghost.reveal received1) (Ghost.reveal sent1) (Ghost.reveal log1) **
+  calc_local_frame_post
+    ev
+    frame
+    result
+    old_out
+    out_contents
+    log0
+    (Ghost.reveal log1)
+    wire_outputs
+    local_outputs **
+  pts_to out out_contents **
+  pure (
+    CPI.local_process_correct
+      CalcP.calc_frame_wire_format_state_machine
+      ev
+      old_out
+      out_contents
+      out_len
+      received0
+      sent0
+      log0
+      result
+      (Ghost.reveal received1)
+      (Ghost.reveal sent1)
+      (Ghost.reveal log1)
+      wire_outputs
+      local_outputs)
+{
+  unfold (canonical_server_exactly srv received0 sent0 log0);
+  unfold (calc_local_frame_pre ev frame log0 out out_len old_out);
+  fold (canonical_server_exactly srv received0 sent0 log0);
+  let local_result = calc_process_result CPI.StepOk 0sz 0sz;
+  fold (calc_local_frame_post ev frame local_result old_out old_out log0 log0 [] []);
+  assert (pure (CPI.local_process_correct
+    CalcP.calc_frame_wire_format_state_machine
+    ev
+    old_out
+    old_out
+    out_len
+    received0
+    sent0
+    log0
+    local_result
+    received0
+    sent0
+    log0
+    []
+    []));
+  local_result
+}
+
+fn new_canonical_server ()
+requires emp
+returns srv:canonical_server
+ensures canonical_server_exactly srv Seq.empty Seq.empty initial_log
+{
+  let server_state = Calc.Server.new_server ();
+  let progress = MR.alloc #_ #calc_server_state_ahead_preorder initial_log;
+  let srv = {
+    canonical_server_state = server_state;
+    canonical_server_progress = progress;
+  };
+  rewrite (server_exactly server_state initial_log) as
+    (server_exactly srv.canonical_server_state initial_log);
+  rewrite (MR.pts_to progress #1.0R initial_log) as
+    (MR.pts_to srv.canonical_server_progress #1.0R initial_log);
+  assert (pure (canonical_trace_witness Seq.empty Seq.empty initial_log empty_calc_trace));
+  assert (pure (canonical_trace_ok Seq.empty Seq.empty initial_log));
+  fold (canonical_server_exactly srv Seq.empty Seq.empty initial_log);
+  srv
+}
+
+noextract
+let calc_server_protocol_implementation
+  : CPI.protocol_implementation
+      canonical_server
+      calc_log
+      CalcP.calc_frame
+      CalcP.calc_frame_local_event
+      unit
+  =
+  {
+    CPI.pi_system = CalcP.calc_frame_wire_format_state_machine;
+    CPI.pi_invariant = canonical_server_exactly;
+    CPI.pi_snapshot = canonical_server_snapshot;
+    CPI.pi_network_frame = calc_network_frame;
+    CPI.pi_network_frame_pre = calc_network_frame_pre;
+    CPI.pi_network_frame_post = calc_network_frame_post;
+    CPI.pi_local_frame = calc_local_frame;
+    CPI.pi_local_frame_pre = calc_local_frame_pre;
+    CPI.pi_local_frame_post = calc_local_frame_post;
+    CPI.pi_invariant_valid = calc_invariant_valid;
+    CPI.pi_take_snapshot = calc_take_snapshot;
+    CPI.pi_recall_snapshot = calc_recall_snapshot;
+    CPI.pi_process_network = calc_process_network;
+    CPI.pi_process_local = calc_process_local;
+  }
